case_study/RiscvPmp/trace.v
@@ -3,9 +3,11 @@ From iris.base_logic Require Import lib.own.
 From iris.proofmode Require Import tactics.
 
 Class traceG (Trace : Type) Σ := TraceG {
-    trace_inG :: inG Σ (authR (optionUR (exclR (leibnizO Trace))));
-    trace_name : gname
-}.
+                                     trace_inG :: inG Σ (authR (optionUR (exclR (leibnizO Trace))));
+                                     trace_name : gname
+                                   }.
+
+
 
 Definition tracePreΣ (Trace : Type) : gFunctors := #[GFunctor (authR (optionUR (exclR (leibnizO Trace))))].
 
@@ -95,3 +97,90 @@ Definition tr_frag1_if `{traceG Σ} (trb : bool) t :=
 Proof.
   intros. rewrite /tr_frag1_if. destruct trb; apply _.
 Qed.
+
+(* iostate *)
+Class iostateG (IOStateG : Type) Σ := IOStateG {
+   iostate_inG :: inG Σ (authR (optionUR (exclR (leibnizO IOStateG))));
+   iostate_name : gname
+}.
+
+
+Definition iostatePreΣ (IOStateG : Type) : gFunctors := #[GFunctor (authR (optionUR (exclR (leibnizO IOStateG))))].
+
+Class iostate_preG (IOState: Type) Σ := {
+    iostate_preG_inG :: inG Σ (authR (optionUR (exclR (leibnizO IOState))));
+  }.
+
+#[export] Instance iostateG_preG `{iostateG T Σ} : iostate_preG T Σ.
+Proof. constructor. typeclasses eauto. Defined.
+
+#[export] Instance subG_iostatePreG{Σ T}:
+  subG (iostatePreΣ T) Σ →
+  iostate_preG T Σ.
+Proof. solve_inG. Qed.
+
+Section S.
+  Context `{!iostate_preG T Σ}.
+  Context (γ : gname). (* To allow using different gnames *)
+
+  Definition st_auth (s: T) : iProp Σ := own γ (● (Some (Excl (s: leibnizO T)))).
+  Definition st_frag (s: T) : iProp Σ := own γ (◯ (Some (Excl (s: leibnizO T)))).
+
+  Lemma iost_full_frag_eq s s':
+    st_auth s -∗ st_frag s' -∗
+    ⌜ s = s' ⌝.
+  Proof.
+    iIntros "H1 H2".
+    iDestruct (own_valid_2 with "H1 H2") as %[Hi Hv]%auth_both_valid_discrete.
+    rewrite Excl_included in Hi.  apply leibniz_equiv in Hi. subst; auto.
+  Qed.
+
+  Lemma st_frag_excl s s' :
+    st_frag s -∗ st_frag s' -∗ ⌜ False ⌝.
+  Proof.
+    iIntros "H1 H2". iDestruct (own_valid_2 with "H1 H2") as %Hv.
+    now apply excl_auth.excl_auth_frag_op_valid in Hv.
+  Qed.
+
+  Lemma state_update s s' :
+    st_auth s ∗ st_frag s ==∗
+    st_auth s' ∗ st_frag s'.
+  Proof.
+    rewrite /st_auth /st_frag. rewrite -!own_op.
+    iApply own_update. apply auth_update.
+    apply option_local_update.
+    apply exclusive_local_update. constructor.
+  Qed.
+
+  #[export] Instance st_auth_Timeless s : Timeless (st_auth s).
+  Proof.
+    intros. apply _.
+  Qed.
+
+  #[export] Instance st_frag_Timeless s : Timeless (st_frag s).
+  Proof.
+    intros. apply _.
+  Qed.
+End S.
+
+Notation st_auth1 := (st_auth iostate_name).
+Notation st_frag1 := (st_frag iostate_name).
+
+
+Lemma state_alloc_names `{!iostate_preG T Σ} s :
+  ⊢ |==> ∃ γ, st_auth γ s ∗ st_frag γ s.
+Proof.
+  iMod (own_alloc (● (Some (Excl (s: leibnizO T))) ⋅ ◯ (Some (Excl (s: leibnizO T))))) as (γ) "[? ?]".
+  { apply auth_both_valid_2; done. }
+  iModIntro. iExists _. iFrame.
+Qed.
+
+Lemma state_alloc `{!iostate_preG T Σ} s :
+  ⊢ |==> ∃ sG : iostateG T Σ,
+
+      @st_auth _ _ (@iostateG_preG _ _ sG) iostate_name s ∗ @st_frag _ _ (@iostateG_preG _ _ sG) iostate_name s.
+Proof.
+  iMod (state_alloc_names s) as (γ) "Hinit".
+  by iExists (IOStateG _ _ _ γ).
+Qed.
+
